\input{../../../template.tex}

\begin{document}
    \begin{enumerate}
      \item
        Here, we use Landin's knot to implement the Fibonacci function.

\begin{verbatim}
let knot f = 
  let r = ref (fun n -> 0) in
  let recur = fun n -> !r n;;
  (r := f recur n);
  recur;;

let fibonacci_fp = fun f n ->
  if n = 0 then 0 else
  if n = 1 then 1 else
  f (n-1) + f (n-2);;

let fibonacci = fun n ->
  (knot fibonacci_fp) n;;
\end{verbatim}

\item
  \begin{enumerate}
    \item

      We give the following typing rule:

      \[
        \frac{\Sigma;\Gamma \vdash e : ref X}{\Sigma;\Gamma \vdash \text{free }e : 1}
      .\] 

      And operational semantics:

      \[
        \frac{\langle \sigma;e \rangle \leadsto \langle \sigma' e' \rangle}{\langle \sigma;\text{free }e \rangle \leadsto \langle \sigma';\text{free }e'\rangle}
      .\] 

      \[
        \frac{l:v \in \sigma}{\langle \sigma; \text{free }l \rangle \leadsto \langle(\sigma \setminus l:v);\langle \rangle \rangle}
      .\] 

    \item
      The issue here is that we break store monotonicity.

      Consider:

      $\langle l : \langle \rangle; \text{free } l\rangle : \langle l: 1 ; 1\rangle$

      We also have:

      $\langle l : \langle \rangle; \text{free } l\rangle \leadsto \langle \cdot ; \langle \rangle \rangle$

      But $\langle \cdot ; \langle \rangle \rangle : \langle \cdot;1\rangle$, and $\cdot \not \geq l:1$, so preservation no longer holds.
  \end{enumerate}
    \end{enumerate}
\end{document}
