\input{../../../template.tex}

\begin{document}

To prove type safety, we prove the following properties: progress and preservation.

In order to do these proofs, we use weakening, exchange, and substitution.

We only prove it for the $\rightarrow I$ rule.

  \begin{enumerate}
    \item
      We begin with weakening.

      We proceed by structural induction.

      We start with the $\rightarrow I$ rule:

      \[
        \frac{\Gamma,\Gamma', x : X \vdash e : Y}{\Gamma,\Gamma' \vdash \lambda x : X. e : X \rightarrow Y}
      .\] 

      We are required to prove that for any $z : T$, $\Gamma, z:T \Gamma' \vdash \lambda x : X. e : X \rightarrow Y$

      We assume that weakening holds for the subderivation  $\Gamma, \Gamma', x : X \vdash e : Y$

      By letting $\Gamma'' = \Gamma', x : X$, we can use weakening to give us $\Gamma, z : T, \Gamma'' \vdash e : Y$, or $\Gamma, z : T, \Gamma', x : X \vdash e : Y$

      Therefore, we can use the $\rightarrow I$ rule to give:

      \[
        \frac{\Gamma, z : T, \Gamma', x : X \vdash e : Y}{\Gamma, z : T, \Gamma' \vdash \lambda x: X. e : X \rightarrow Y}
      .\] 

      We now consider the $\rightarrow E$ case.

      We have:

      \[
        \frac{\Gamma,\Gamma' \vdash e : X \rightarrow Y \hspace{15pt} \Gamma, \Gamma' \vdash e' : X}{\Gamma, \Gamma' \vdash e e' : Y}
      .\] 

      We assume we have weakening on our subderivations, so we can simply apply the $\rightarrow E$ rule again:

      \[
        \frac{\Gamma, x : T, \Gamma' \vdash e : X \rightarrow Y \hspace{15pt} \Gamma, x : T, \Gamma' \vdash e' : X}{\Gamma, x : T, \Gamma' \vdash e e' : Y}
      .\] 

      We now consider the $1I$ case.

      We have:

      \[
        \frac{}{\Gamma,\Gamma' \vdash \langle \rangle : 1}
      .\] 

      Using the same rule, we get:

      \[
        \frac{}{\Gamma, x : T, \Gamma' \vdash \langle \rangle : 1}
      .\] 

      So we are done.

    \item
      We now prove exchange.

      Again, we use structural induction.

      We begin with the $\rightarrow I$ case.

      So, we have:

      \[
        \frac{\Gamma, y : T, y': T', \Gamma', x : X \vdash e : Y}{\Gamma, x : T, x' : T', \Gamma' \vdash \lambda x : X. e : X \rightarrow Y}
      .\] 

      We are required to prove that $\Gamma, x : T, x' : T', \Gamma' \vdash \lambda x : X. e : X \rightarrow Y$

      We assume we have exchange on the subderivation $\Gamma, y : T, y' : T', \Gamma', x : X \vdash e : Y$

      Therefore, by letting $\Gamma'' = \Gamma', x : X$, through exchange we get $\Gamma, y' : T, y : T, \Gamma'' \vdash e : Y$, or $\Gamma, y' : T', y : T, \Gamma', x : X \vdash e : Y$

      Therefore, we use the $\rightarrow I$ rule to get:

      \[
        \frac{\Gamma, y': T', y : T, \Gamma', x : X \vdash e : Y}{\Gamma, y' : T', y : T, \Gamma ' \vdash \lambda x : X. e : X \rightarrow Y}
      .\] 

      We now consider the $\rightarrow E$ case:

      So, we have:

      \[
        \frac{\Gamma, y : T, y' : T', \Gamma' \vdash e : X \rightarrow Y \hspace{15pt} \Gamma, y : T, y' : T', \Gamma' \vdash e' : X}{\Gamma, y : T, y' : T', \Gamma' \vdash e e' Y}
      .\] 

      We assume we have exchange on the subderivations, so we immediately get, using the $\rightarrow E$ rule,:

      \[
        \frac{\Gamma, y' : T', y : T, \Gamma' \vdash e : X \rightarrow Y \hspace{15pt} \Gamma, y' : T', y : T, \Gamma' \vdash e' : X}{\Gamma, y' : T', y : T, \Gamma' \vdash e e' : Y}
      .\] 

      We now consider the $1I$ case:

      We have:

      \[
        \frac{}{\Gamma, y : T ,y' : T',  \Gamma' \vdash \{\} : 1}
      .\] 

      We use the $1I$ rule immediately to get:

      \[
        \frac{}{\Gamma, y': T', y : T, \Gamma' \vdash \{\} : 1}
      .\] 

      So, we are done.

    \item
      We now prove substitution.

      Again, we use structural induction.

      We first consider the $\rightarrow I$ case:

      So, we have:

      \[
        \frac{\Gamma, y : T, x : X \vdash e : Y}{\Gamma, y : T \vdash \lambda x : X. e : X \rightarrow Y}
      .\] 

      Our subderivation gives us $\Gamma, y : T, x : X \vdash e : Y$, and by exchange we know this is equivalent to $\Gamma, x : X, y : T \vdash e : Y$. We assume we have substitution on both.

      Therefore, if we have a term $e'$ such that $\Gamma, \vdash e' : T$, then by weakening we know that $\Gamma, x : X \vdash e' : T$, and so we can apply substitution to give us $\Gamma, x : X \vdash [e' / y]e : Y$

      Therefore, we apply the $\rightarrow I$ rule to get:

      \[
        \frac{\Gamma, x : X \vdash [e' / y]e : Y}{\Gamma \vdash \lambda x : X. [e' / y]e : X \rightarrow Y}
      .\] 


      From the definition of substitution, we know that $[e' / y](\lambda x: X . e) = \lambda x : X . [e' / y]e$, so therefore we have $\Gamma \vdash [e' / y](\lambda x : X . e) : X \rightarrow Y$, as required.

      We now consider the $\rightarrow E$ case:

      So, we have:

      \[
        \frac{\Gamma, y : T \vdash e : X \rightarrow Y \hspace{15pt} \Gamma, y : T \vdash e' : X}{\Gamma, y : T \vdash e e' : X \rightarrow Y}
      .\] 

      We assume we have $e''$ such that $\Gamma \vdash e'' : T$. We assume we have substitution on our subderivations, i.e. that $\Gamma \vdash [e'' / y]e : X \rightarrow Y$ and $\Gamma \vdash [e'' / y]e' : X$.

      Therefore, using the $\rightarrow E$ rule again, we get:

      \[
        \frac{\Gamma \vdash [e'' / y]e : X \rightarrow Y \hspace{15pt} \Gamma \vdash [e'' / y]e' : X}{\Gamma \vdash [e'' / y]e [e'' / y]e' : X \rightarrow Y}
      .\] 

      By definition of substitution, we know $[e'' / y]e [e'' / y]e' = [e'' / y](e e')$, so we therefore get $\Gamma \vdash [e'' / y](e e') : X \rightarrow Y$ as required.

      We now consider the $1I$ case:

      So, we have:

      \[
        \frac{}{\Gamma, y : T \vdash \langle\rangle : 1}
      .\] 

      Assume we have some $e'$ such that $\Gamma \vdash e' : T$

      From the definition of substitution, and the $1I$ rule, we get:

      \[
        \frac{}{\Gamma \vdash [e' / y]\langle\rangle : 1}
      .\] 

      So we are done.

    \item
      We now prove progress.

      We prove progress with structural induction over typing derivations, as before.

      We begin with the $\rightarrow I$ case.

      So, we have:

      \[
        \frac{x : X \vdash e : Y}{\{\} \vdash \lambda x : X. e : X \rightarrow Y}
      .\] 

      By definition, $\lambda x : X .e$ is a value, so we are done.

      We now proceed with the $\rightarrow E$ case.

      So, we have:

      \[
        \frac{\{\} \vdash e : X \rightarrow Y \hspace{15pt} \{\} \vdash e' : X}{\{\} \vdash e e' : Y}
      .\] 

      We assume we have progress on the subderivations.

      We proceed by cases:

      \begin{itemize}
        \item
          Case $e$ is not a value.

          In this case, we have some $e_1$ such that $e \leadsto e_1$

          Then, we simply use the congruence rule:

          \[
            \frac{e \leadsto e_1}{e e' \leadsto e_1 e'}
          .\] 

          So we have progress.

        \item
          Case $e$ is a value $v_1$.

          We again proceed by cases:

          \begin{itemize}
            \item
              Case $e'$ is not a value.

              In this case, we have some $e_2$ such that $e \leadsto e_2$

              Then, we simply use the congruence rule:

              \[
                \frac{e' \leadsto e_2}{v_1 e' \leadsto v_1 e_2}
              .\] 

              So we have progress.

            \item
              Case $e'$ is a value $v_2$

              Since $v_1$ is well typed, it must be of the form $(\lambda x: X . e'')$.

              Therefore, we use the congruence rule:

              \[
                \frac{}{(\lambda x : X. e'') v_2 \leadsto [v_2 / x]e''}
              .\] 

              So we have progress.
          \end{itemize}
      \end{itemize}

      Therefore we have progress in this case.

      For the $1I$ rule, $\langle\rangle$ is immediately a value so we have progress.

    \item
      We now prove type preservation.

      We proceed by structural induction over reduction this time.

      We only have to deal with functions, since unit never reduces.

      \begin{itemize}
        \item
          We start with the left congruence rule:

          \[
            \frac{e_1 \leadsto e_1'}{e_1 e_2 \leadsto e_1' e_2}
          .\] 

          And we assume $e_1 e_2$ is well-typed, and by deconstructing the typing relation we must have:

          \[
            \frac{\{\} \vdash e_1 : X \rightarrow Y \hspace{15pt} \{\} \vdash e_2 : X}{\{\} \vdash e_1 e_2 : Y}
          \] 

          We assume we have preservation on our subderivation $e_1 \leadsto e_1'$, and since we know that $\{\} \vdash e_1 : X \rightarrow Y$, we use preservation to get $\{\} \vdash e_1' : X \rightarrow Y$

          Therefore, we use the $\rightarrow E$ rule to get:

          \[
            \frac{\{\} \vdash e_1' : X \rightarrow Y \hspace{15pt} \{\} \vdash e_2 : X}{\{\} \vdash e_1' e_2 : Y}
          .\] 

          And so we have preservation in this case.

        \item
          We now consider the right congruence rule:

          \[
            \frac{e_2 \leadsto e_2'}{v_1 e_2 \leadsto v_1 e_2'}
          .\] 

          And we assume $v_1 e_2$ is well-typed, and so we get:

          \[
            \frac{\{\} \vdash v_1 : X \rightarrow Y \hspace{15pt} \{\} \vdash e_2 : X}{\{\} \vdash v_1 e_2 : Y}
          .\] 

          We assume we have preservation on our subderivation $e_2 \leadsto e_2'$, and since we know $\{\} \vdash e_2 : X$, we use preservation to get $\{\} \vdash e_2' : X$

          Therefore, we use the $\rightarrow E$ rule to get:

          \[
            \frac{\{\} \vdash v_1 : X \rightarrow Y \hspace{15pt} \{\} \vdash e_2' : X}{\{\} \vdash v_1 e_2' : Y}
          .\] 

          And so we have preservation in this case.

        \item
          We now consider the actual reduction rule:

          \[
            \frac{}{(\lambda x : X . e) v \leadsto [v / x]e}
          .\] 

          We also assume $(\lambda x : X . e) v$ is well typed, and so that:

          \[
            \frac{\{\} \vdash (\lambda x : X . e) :X \rightarrow Y \hspace{15pt} \{\} \vdash v : X}{\{\} \vdash (\lambda x : X . e) v : Y}
          .\] 

          Again, we deconstruct the typing relation for functions and realise that $\{\} \vdash (\lambda x : X . e ) :X \rightarrow Y$ must come from the typing derivation:

          \[
            \frac{x : X \vdash e : Y}{\{\} \vdash (\lambda x : X . e) : X \rightarrow Y}
          .\] 

          Finally, since we have $x : X \vdash e : Y$, and $\{\} \vdash v : X$, we can use substitution to get $\{\} \vdash [v / x]e : Y$

          So, we have typing preservation in this case.
      \end{itemize}

      So, we have typing preservation.


  \end{enumerate}
\end{document}
